verified/bitvectors.s.dfy
@@ -1,0 +1,115 @@
+lemma {:axiom} lemma_BitvecToInt(b:bv32)
+    ensures 0 <= b as int < 0x1_0000_0000;
+    ensures (b as int) as bv32 == b;
+    ensures b == 0 <==> b as int == 0;
+
+lemma {:axiom} lemma_BitvecIntEquivalence(b:bv32, i:int)
+    requires i == b as int || (0 <= i < 0x1_0000_0000 && b == i as bv32)
+    ensures i == b as int && b == i as bv32
+
+lemma {:axiom} lemma_BitvecIntCasts(b:bv32)
+    ensures b == b as int as bv32
+
+lemma {:axiom} lemma_IntBitvecCasts(i:int)
+    requires 0 <= i < 0x1_0000_0000
+    ensures i == i as bv32 as int
+
+lemma {:axiom} lemma_IntToBitvec(i:int)
+    requires 0 <= i < 0x1_0000_0000;
+    ensures (i as bv32) as int == i;
+    ensures i == 0 <==> i as bv32 == 0;
+
+function IntToBitvec(i:int): bv32
+    requires 0 <= i < 0x1_0000_0000;
+    ensures i == 0 <==> IntToBitvec(i) == 0;
+    ensures IntToBitvec(i) as int == i;
+{
+    lemma_IntToBitvec(i); i as bv32
+}
+
+function BitvecToInt(b:bv32): int
+    ensures 0 <= BitvecToInt(b) < 0x1_0000_0000;
+    ensures b == 0 <==> BitvecToInt(b) == 0;
+    ensures BitvecToInt(b) as bv32 == b;
+    decreases b as int // XXX: workaround Dafny issue #26
+{
+    lemma_BitvecToInt(b); b as int
+}
+
+lemma {:axiom} lemma_BitwiseModEquiv(x:bv32, y:bv32)
+    requires y != 0
+    ensures BitvecToInt(x % y) == BitvecToInt(x) % BitvecToInt(y);
+
+lemma {:axiom} lemma_BitwiseDivEquiv(x:bv32, y:bv32)
+    requires y != 0
+    ensures BitvecToInt(x / y) == BitvecToInt(x) / BitvecToInt(y);
+
+lemma {:axiom} lemma_BitwiseMulEquiv(x:bv32, y:bv32)
+    ensures BitvecToInt(x * y) == BitvecToInt(x) * BitvecToInt(y);
+
+function pow2(n:nat): nat
+    ensures pow2(n) > 0
+{
+    if n == 0 then 1 else 2 * pow2(n - 1)
+}
+
+function BitposValue'(bitpos:int): bv32
+    requires 0 <= bitpos < 32
+{
+    (1 as bv32 << bitpos)
+}
+
+lemma {:axiom} lemma_BitposPowerOf2(bitpos:int)
+    requires 0 <= bitpos < 32
+    ensures BitvecToInt(BitposValue'(bitpos)) == pow2(bitpos)
+
+function BitposValue(bitpos:int): bv32
+    requires 0 <= bitpos < 32
+    ensures BitposValue(bitpos) != 0
+    ensures BitposValue(bitpos) as int == pow2(bitpos)
+{
+    lemma_BitposPowerOf2(bitpos); BitposValue'(bitpos)
+}
+
+function BitmaskLow(bitpos:int): bv32
+    requires 0 <= bitpos < 32
+{
+    BitposValue(bitpos) - 1
+}
+
+function BitmaskHigh(bitpos:int): bv32
+    requires 0 <= bitpos < 32
+{
+    !BitmaskLow(bitpos)
+}
+
+lemma {:axiom} lemma_BitwiseMask(x:bv32, bitpos:int)
+    requires 0 <= bitpos < 32
+    ensures x & BitmaskLow(bitpos) == x % BitposValue(bitpos)
+    ensures x & BitmaskHigh(bitpos) == x / BitposValue(bitpos) * BitposValue(bitpos)
+    ensures (x & BitmaskHigh(bitpos)) % BitposValue(bitpos) == 0
+/* TODO: can't we prove this? */
+
+lemma lemma_BitwiseMaskInt(i:int, bitpos:int)
+    requires 0 <= i < 0x1_0000_0000;
+    requires 0 <= bitpos < 32
+    //ensures BitvecToInt(IntToBitvec(i) & BitmaskLow(bitpos)) == i % pow2(bitpos)
+    //ensures BitvecToInt(IntToBitvec(i) & BitmaskHigh(bitpos)) == i / pow2(bitpos) * pow2(bitpos)
+    ensures BitvecToInt(IntToBitvec(i) & BitmaskHigh(bitpos)) % pow2(bitpos) == 0
+{
+    lemma_BitwiseMask(IntToBitvec(i), bitpos);
+    assert (IntToBitvec(i) & BitmaskHigh(bitpos)) % BitposValue(bitpos) == 0;
+    lemma_BitwiseModEquiv(IntToBitvec(i) & BitmaskHigh(bitpos), BitposValue(bitpos));
+    assert BitvecToInt(BitposValue(bitpos)) == pow2(bitpos);
+}
+
+function BitwiseMaskHighBitsInt(i:int, bitpos:int): int
+    requires 0 <= i < 0x1_0000_0000;
+    requires 0 <= bitpos < 32;
+    ensures 0 <= BitwiseMaskHighBitsInt(i, bitpos) < 0x1_0000_0000;
+    ensures BitwiseMaskHighBitsInt(i, bitpos) % pow2(bitpos) == 0
+{
+    lemma_BitwiseMaskInt(i, bitpos);
+    assert BitvecToInt(IntToBitvec(i) & BitmaskHigh(bitpos)) % pow2(bitpos) == 0;
+    BitvecToInt(IntToBitvec(i) & BitmaskHigh(bitpos))
+}
